\documentclass[a4paper,12pt]{article}


\usepackage{ProfModels}

 
\begin{document}

\begin{Maquette}[Fiche]{Theme=Calcule littéral,Niveau=2}



\begin{exercice}
Réduire les expressions suivantes :
\[
A=2x-\left(1+5a+4x-\left(7x-2a+7\right)-4\right)\quad ;; \quad
B=-5a-7x+5x^{2}-2x+3x^{2}
\]
\[
C=5-\left(3+4x-2y\right)+\left(5-2y+8x\right)\quad ;; \quad
D=8a^{3}-5+5a\times 6a-6a^{3}+9
\]
\end{exercice}

\begin{exercice}
Développer et réduire :
\[
A=2\left(1-4x\right)+3x\left(2x+2\right)\quad ;; \quad
B=-4x\left(-2x+6\right)-5x\left(3x-4\right)
\]
\[
C=\left(2x+5\right)\left(x-3\right)-5\left(2x-3\right)\quad ;; \quad
D=\left(5x+8\right)\left(3x-7\right)+\left(2x-1\right)\left(3x-7\right)
\]
\[
E=2x^{2}\left(6x^{3}-7x^{5}\right)\quad ;; \quad
F=\left(-6x-3\right)\left(2x-7\right)
\]
\end{exercice}

\begin{exercice}
Développer et réduire :
\[
M=\left(6x+7\right)^{2}\quad ;; \quad
N=\left(2x-6\right)^{2}\quad ;; \quad
P=\left(7x-1\right)\left(7x+1\right)\quad ;; \quad
Q=\left(\dfrac{5x}{7}-8\right)\left(\dfrac{5x}{7}+8\right)
\]
\[
A=2x\left(1-4x\right)+3x\left(2x+2\right)\quad ;; \quad
B=-4x\left(-2x-3\right)-5x\left(3x-1\right)
\]
\[
C=\left(\dfrac{x}{4}-1\right)\left(\dfrac{-2x}{3}+1\right)-\dfrac{1}{6}x^{2}\left(1-x\right)\quad ;; \quad
D=\left(\dfrac{2}{5}x-3\right)\left(-2x^{2}+x-1\right)-2x^{2}\left(\dfrac{x}{5}-4\right)
\]
\end{exercice}

\begin{exercice}
Compléter par ce qui convient :
\[
\left(\cdots + 2\right)^{2}=9x^{2}+\cdots +4 \quad ;; \quad
\left(5x+\cdots\right)^{2}=\cdots + \cdots +9
\]
\[
\left(\cdots - \dfrac{1}{2}\right)^{2}=\dfrac{9}{4}x^{2}-\cdots +\cdots\quad ;; \quad
\left(\cdots - \cdots \right)^{2}=\cdots - 56x+16
\]
\[
\left(\cdots +\cdots\right)\left(\cdots - \cdots\right)=\dfrac{1}{4}-\dfrac{25}{9}x^{2}\quad ;; \quad
\left(\dfrac{9}{4}x-\cdots\right)\left(\cdots + \cdots\right)=\cdots - 81
\]
\[
\left(\dfrac{3}{5}+\cdots\right)\left(\cdots -\dfrac{9}{7}x\right)=\cdots - \cdots\quad ;; \quad
\left(\cdots - \dfrac{2}{3}\right)\left(5x+\cdots\right)=\cdots - \cdots
\]
\end{exercice}

\begin{exercice}
Développer et réduire :
\[
A=\left(2x-1\right)^{2}\quad ;; \quad
B=\left(-3x-5\right)^{2}\quad ;; \quad
C=\left(3x-4\right)\left(3x+4\right)\quad ;; \quad
D=-2x\left(3-x\right)^{2}
\]
\[
E=\left(2x-1\right)^{2}+\left(3x-1\right)-2x\left(x+3\right)\quad ;; \quad
F=\left(3x-1\right)\left(3x+1\right)-2x\left(5x+4\right)-\left(-x-3\right)
\]
\[
G=\left(x+\dfrac{2}{3}\right)^{2}+\left(\dfrac{3}{2}x-4\right)^{2}-\left(\dfrac{3}{2}x-2\right)\left(\dfrac{3}{2}x+2\right)\quad ;; \quad
H=\left(\dfrac{5}{2}x-2\right)^{2}-\left(3x+1\right)\left(\dfrac{1}{2}x-2\right)
\]
\[
I=\dfrac{3}{2}x\left(-x+1\right)^{2}+\dfrac{2}{3}x\left(-\dfrac{1}{2}x-3\right)\left(-\dfrac{1}{2}x+3\right)\quad ;; \quad
J=2x^{2}\left(\dfrac{1}{2}-x\right)\left(\dfrac{1}{2}+x\right)-\dfrac{3}{5}x\left(x-2\right)^{2}
\]
\end{exercice}

\begin{exercice}
Factoriser :
\[
a=5x\left(3x-2\right)+5x\left(-2x+1\right)\quad ;; \quad
b=3x^{2}+3x\left(2x-5\right)-3x\quad ;; \quad
c=12x^{3}+4x^{2}\left(x+3\right)-4x^{2}
\]
\[
d=3x\left(2x-1\right)-\left(2x-1\right)\quad ;; \quad
e=5x\left(3-x\right)+\left(3-x\right)^{2}
\]
\[
f=\left(1-x\right)\left(x+1\right)-\left(1-x\right)^{2}+\left(1-x\right)
\]
\[
g=\left(\dfrac{5}{2}x-1\right)\left(x-\dfrac{3}{2}\right)+2\left(\dfrac{5}{2}x-1\right)-\dfrac{4}{3}x\left(\dfrac{5}{2}x-1\right)\quad ;; \quad
i=\left(\dfrac{x}{7}+3\right)^{2}-\left(\dfrac{2x}{7}+6\right)
\]
\[
h=2x\left(\dfrac{3}{5}x-\dfrac{1}{2}\right)+4x\left(\dfrac{3}{5}x-\dfrac{1}{2}\right)-\left(\dfrac{3}{5}x-\dfrac{1}{2}\right)
\]
\[
j=-3x\left(\dfrac{-2}{5}x-1\right)+3x\left(5-\dfrac{3}{5}x\right)-9x^{2}\quad ;; \quad
k=-\dfrac{5}{7}x\left(\dfrac{2x}{5}+1\right)+\left(\dfrac{6x}{5}+3\right)
\]
\end{exercice}

\begin{exercice}
Factoriser :
\[
A=25x^{2}+20x+4\quad ;; \quad
B=9+12x+4x^{2}\quad ;; \quad
C=81-36x+4x^{2}
\]
\[
D=16x^{2}-56x+49\quad ;; \quad
E=16x^{2}-9\quad ;; \quad
F=144-4x^{2}
\]
\[
G=\dfrac{16}{9}x^{2}+\dfrac{16}{9}x+\dfrac{4}{9}\quad ;; \quad
H=9x^{2}-\dfrac{9}{2}x+\dfrac{9}{16}
\]
\end{exercice}

\end{Maquette}

\end{document}