\documentclass[a4paper,12pt]{article}


\usepackage{ProfModels}

 
\begin{document}
\begin{Maquette}[Fiche]{Theme=Développement et factorisation,présentation}


\begin{exercice}
Réduire ce qui suit :
\[
A=5x-2x^{2}+7x-3x^{2}+7\quad ;; \quad
B=3x-(2x^{2}+3x-5x^{2}-1)+x^{2}-1
\]
\[
C=-(5x-2x^{2}+4)-(-5x-2x^{2}+5)-8\quad ;; \quad
D=3ab-6+7ab+9a^{2}b
\]
\end{exercice}

\begin{exercice}
Développer et réduire ce qui suit :
\[
A=2x(3x+1)\quad ;; \quad
B=3x(2-5x)\quad ;; \quad
C=-x^{2}(-4x^{2}+5)\quad ;; \quad
D=-5x^{5}(-4x+2x^{3})
\]
\[
E=5x(x^{5}-2x^{3}+x-7)\quad ;; \quad
F=-7x^{3}(2x^{2}-7x+3x^{8}-8)
\]
\[
G=(2x+3)(5x+8)\quad ;; \quad
H=(5x-4)(9x-7)\quad ;; \quad
I=(8x-1)(4x+9)
\]
\end{exercice}

\begin{exercice}
Développer et réduire ce qui suit :
\[
A=(3x+5)^{2}\quad ;; \quad
B=(5x-3)^{2}\quad ;; \quad
C=(5x-9)(5x+9)
\]
\[
D=(3x-1)^{2}-(7x+2)^{2}+(8x+1)(8x-1) \quad ;;\quad
E=(4x-1)^{2}-(5-x)^{2}
\]
\[
F=3x^{3}(x-1)(x+1)+2x^{2}(x-1)^{2}-4x(x+1)^{2}
\]
\end{exercice}

\begin{exercice}
Factoriser les expressions suivantes :
\[
5x-25\quad ;; \quad
17a+51\quad ;; \quad
ab^{2}+(ab)^{2}-a^{2}b
\]
\[
(2x+1)(x+1)+5(x+1)\quad ;; \quad
(8a+7)(3b-1)-7(8a+7)+8a+7
\]
\[
5x^{2}+2x+7x^{3}\quad ;; \quad
49a+7b-21\quad ;; \quad
121x+66y-11
\]
\[
18ab+24xy\quad ;; \quad
45x^{2}-65y^{2}+25
\]
\[
4x^{2}(x-9)+(3x-7)(x-9)+4x(x-9)(5x+7)+x-9
\]
\end{exercice}
\begin{exercice}
Factoriser les expressions suivantes :

$$3(x+3)(2x-1)-(3x-4)(4x-2) $$
$$6x^{3}(6x-9)-7(2x-3) $$
$$(8x-24)+(3x-7)(x-3) $$
$$9x+3+7x(2x+3)(6x+2)$$

\end{exercice}
\end{Maquette}
\end{document}